Makefile
@@ -1,0 +1,2 @@
+all:
+	~/Isabelle2014/bin/isabelle build -o quick_and_dirty -D .
